src/coq/Dot_Transitivity.v
@@ -111,16 +111,4 @@ assert (E |= S' ~<: tp_sel t l) as Ht1; eauto 3.
 assert (E |= tp_sel t l ~<: U') as Ht2; eauto 3.
 skip. (* TODO *)
 
-assert (E |= S' ~<: tp_sel t l) as Ht1; eauto 3.
-assert (E |= tp_sel t l ~<: T) as Ht2; eauto 3.
-skip. (* TODO *)
-
-assert (E |= T ~<: tp_sel t l) as Ht1; eauto 3.
-assert (E |= tp_sel t l ~<: U') as Ht2; eauto 3.
-skip. (* TODO *)
-
-assert (E |= T ~<: tp_sel t l) as Ht1; eauto 3.
-assert (E |= tp_sel t l ~<: T0) as Ht2; eauto 3.
-skip. (* TODO *)
-
 Qed.
